\documentclass{article}
\input{setup.tex}


\renewcommand*\contentsname{Table of Content}

\title{Complex Function Theory}
\author{Mattie Ji}
\date{Updated \today}

\begin{document}

\maketitle

\noindent Technically, this is a course on ``functions of ONE complex variable".
\tableofcontents
\newpage

\include{Lecture/lecture-1.tex}
\include{Lecture/lecture-2.tex}
\include{Lecture/lecture-3.tex}
\include{Lecture/lecture-4.tex}
\include{Lecture/lecture-5.tex}
\include{Lecture/lecture-6.tex}


\newpage
\section{Lecture 7}

\subsection{Revisiting Exponential}

\begin{definition}
    Let $z \in \Cbb$, we define the complex exponential map $e^z: \Cbb \to \Cbb$ as
    \[e^z \coloneqq 1 + z + \frac{z^2}{2!} + ... = \sum_{n = 0}^\infty \frac{z^n}{n!}\]
\end{definition}

\begin{theorem}[Euler's Identity]
Let $x \in \Rbb$, then
\[e^{ix} = cos(x) + i sin(x)\]
\end{theorem}

\begin{proof}
We can show this via explicit computation, indeed,
\begin{align*}
    e^{ix} &= \sum_{n = 0}^\infty \frac{(ix)^n}{n!}\\
    &= \sum_{k = 0}^\infty (-1)^k \frac{x^{2k}}{(2k)!} + i \sum_{k = 0} (-1)^k \frac{x^{2k + 1}}{(2k + 1)!} \tag*{Separate even and odd degree terms}\\
    &= cos(x) + i sin(x) \tag*{Taylor Series}
\end{align*}
\end{proof}

\begin{lemma}\label{lem::real_analy_fact}
Facts from Analysis:
\begin{enumerate}
    \item For every $r \in \Rbb$, $\sum_{n = 0}^\infty \frac{r^n}{n!}$ converges absolutely
    \item If $a_n \in \Cbb$ and $\sum_{n = 0}^\infty |a_n|$ converges, then $\sum_{n = 0}^\infty a_n$ converges
    \item If $L_a = \sum_{n = 0}^\infty a_n, L_b = \sum_{m = 0}^\infty b_m$ converges absolutely, then
    \[\sum_{n = 0}^\infty \sum_{k = 0}^n a_k b_{n - k}\]
    converges to
    \[(\sum_{n = 0}^\infty a_n) \cdot (\sum_{m = 0}^\infty b_m)\]
\end{enumerate}
This will helpful in proving some identities.
\end{lemma}

\begin{proof}
For $(1)$, we will use the ratio test. Indeed, consider $a_n = \frac{r^n}{n!}$, then
\[\lim_{n \to \infty} |\frac{a_{n+1}}{a_n}| = \lim_{n \to \infty} |\frac{r}{n + 1}| = 0 < 1\]
Thus, the series converges absolutely.\\\\
For $(2)$, let $b_n = \sum_{i = 1}^n a_i, c_n = \sum_{i = 1}^n |a_i|$. We note that the topology $\Cbb$ is homeomorphic to the Euclidean topology on $\Rbb^2$, so in particular $\Cbb$ is a complete metric space, so a sequence is convergent if and only if it is Cauchy. We know $c_n$ converges, so for every $\epsilon > 0$, there exists some $N_c$ such that for all $i, j > N_c$.
\[|c_i - c_j| < \epsilon\]
It remains for us to show that $b_n$ is also Cauchy. Indeed, if $i = j$, then we are done. Without loss, we will then assume $j > i$, then
\begin{align*}
    |b_i - b_j| &= |\sum_{k = i + 1}^j a_k|\\
    &\leq \sum_{k = i + 1}^j |a_k| \tag*{Triangle's Inequality}\\
    &= |c_i - c_j|\\
    &< \epsilon
\end{align*}
Thus, $\{b_n\}$ is Cauchy and converges.\\\\
For $(3)$, $(\sum_{n = 0}^\infty a_n) \cdot (\sum_{m = 0}^\infty b_m)$ certainly converges to $L_a \cdot L_b$. Now write $(\sum_{n = 0}^\infty a_n) \cdot (\sum_{m = 0}^\infty b_m) = \sum_{n = 0}^\infty \sum_{m = 0}^\infty a_n b_m$, this corresponds exactly to the terms of $\sum_{n = 0}^\infty \sum_{k = 0}^n a_k b_{n - k}$. The exact combinatorics is left as details to the reader.
\end{proof}

\begin{corollary}
Let $e^z$ be the complex exponential map, then
\begin{itemize}
    \item $e^z$ converges for all $z \in \Cbb$
    \item $e^{z + w} = e^z \cdot e^w$ for all $z, w \in \Cbb$
\end{itemize}
\end{corollary}

\begin{proof}
For the first, let $a_n = \sum_{k = 1}^n |\frac{z^k}{k!}|$. It suffices for us to prove that $a_n$ converges as absolute convergence implies monotone convergence from Lemma~\ref{lem::real_analy_fact}(2). But we note that 
\[|\frac{z^k}{k!}| = \frac{|z|^k}{k!}\]
and $|z|$ is a real number, so Lemma~\ref{lem::real_analy_fact}(1) tells us that $a_n$ converges.\\\\
For the second, we note that
\begin{align*}
    e^{z + w} &= \sum_{n = 0}^\infty \frac{(z + w)^n}{n!}\\
    &= \sum_{n = 0}^\infty \sum_{k = 0}^n {n \choose k} \frac{z^k w^{n-k}}{n!} \tag*{Binomial Theorem}\\
    &= \sum_{n = 0}^\infty \sum_{k = 0}^n \frac{z^k}{k!} \frac{w^{n-k}}{(n - k)!}\\
    &= (\sum_{n = 0}^\infty \frac{(z)^n}{n!}) \cdot (\sum_{n = 0}^\infty \frac{(w)^n}{n!}) \tag*{By Lemma~\ref{lem::real_analy_fact}(3)}\\
    &= e^z \cdot e^w
\end{align*}
\end{proof}

\begin{proposition}
We can also recover $\cos(z)$ and $\sin(z)$ from $e^z$ as
\[\cos(z) = \frac{e^{iz} + e^{-iz}}{2}, \sin(z) = \frac{e^{iz} - e^{-iz}}{2i}\]
If $x \in \Rbb$, we also have that
\[\cos(x) = \Re e^{ix}, \sin(x) = \Im e^{ix}\]
\end{proposition}

\subsection{Complex Logarithms}

As in the case of $\Rbb$, we want to define $\log(z)$ as an inverse to $e^z$ such that
\[e^{\log(z)} = z\]
The problem is that $e^z$ is not actually injective, so there are multiple choices for $\log(z)$. Consequently, this will result in $\log(z)$ not being continuous on all of $\Cbb$.

\begin{question}
Given $z$, can we find all solutions satifying $e^w = z$?
\end{question}

\begin{proof}[Answer]
We will again leverage on Polar Coordinates. Indeed, write $z = re^{i \theta}, w = x + iy$, then we have that
\[r e^{i \theta} = e^{x + iy} = e^{x} e^{iy}\]
Thus, $x = \log(r), y = \theta + 2 \pi k$.\\\\
Thus, $w$ is of the form $w_k = \log(r) + i(\theta + 2 \pi k)$
\end{proof}

\begin{definition}[Complex Logarithm]
    For $z \in \Cbb \setminus \{0\}$, write $z = re^{i \theta}, \theta \in [-\pi, \pi]$. Then we define
    \[\log(z) = \log(r e^{i \theta}) \coloneqq \log(r) + i \theta\]
    $\theta$ is sometimes refered to as the \textbf{principal argument} of $z$ and we denote $Arg(z) = \theta$.
\end{definition}

\begin{remark}
Note that the complex logarithm $\log(z)$ is not continuous on all of $\Cbb$:
\[\includegraphics[width=0.5\textwidth]{Figures/complex_log.png}\]
As you trace around the unit circle, going back to $z = 1$ presents a problem.\\\\
Therefore, we can only define the complex logarithm up to a \textbf{branch cut} that's a radial line extending out from the origin. We will without loss choose this branch to be $(-\infty, 0]$
\end{remark}

\begin{proposition}
$\log(z)$ is holomorphic on $\Cbb \setminus (-\infty, 0]$ and in fact $\frac{d}{dz} \log(w) = \frac{1}{w}$
\end{proposition}

\begin{proof}
One way to do this is to use the Cauchy-Riemann equations in polar coordinates. We will however use the Inverse Function Theorem instead. Indeed, we note that on $\Cbb \setminus (-\infty, 0]$, $z \mapsto e^z$ is a smooth function with non-zero derivatives, so the inverse function theorem tells us that $\log(z)$ is also holomorphic. Furthermore, locally for all $w = e^z \in \Cbb \setminus (-\infty, 0]$,
\[\frac{d}{dz} \log(w) = \frac{1}{e^z} = \frac{1}{w}\]
\end{proof}

\noindent Note that we didn't define the Inverse Function Theorem for complex variables, but we treated the map $z \to e^z$ as a function of two variables from $\Rbb^2$ to $\Rbb^2$.

\begin{remark}
Let $z \in \Cbb \setminus (-\infty, 0]$, then since $\frac{1}{z}$ is primitive on the path $1$ to $z$, we have that:
\[\int_1^z \frac{d\xi}{\xi} = \log(z) - \log(1) = \log(z)\]
\end{remark}

\subsection{Homotopy Invariance of Integral}

Let $f \in \Hol(\Omega)$ and $\gamma: [a, b] \to \Gamma$ is continous and $\Gamma \subset \Omega$, then we can define the integral
\[\int_\gamma f(z) dz\]

Informally, we can define this because at each point on $\gamma$, we can find some disk to represent $f$ as a power series with a primitive $F$, then we can split $[a, b]$ into a union of (not necessarily uniform) subintervals, then the integral $\gamma$ can be approximated as a sum of the anti-derivatives $F_k$ at each end-points.

We can formally justify this with what's called the Lebesgue's Number Lemma.

\begin{lemma}[Lebesgue's Number Lemma]
Let $K$ be a compact metric space and let $\{U_a\}$ be an open cover for $K$, then there exists some $\delta > 0$ (we call the \textbf{Lebesgue Number}) such that for all $x \in K$, there exists some $a$ such that $B_{x, \delta} \subset U_a$
\end{lemma}

\mattie{Work in progress}
\begin{proof}
For all $x \in K$, since $\{U_a\}$ is an open cover of $K$, there exists some $a$ such that $x \in U_a$. Since $U_a$ is open, there exists some $r(x) > 0$ small enough such that $B_{x, 2r(x)} \subset U_\alpha$.\\\\
Note that $\{B_{x, 2r(x)}\}$ running over all $x \in K$ is an open cover of $K$. Since $K$ is compact, we in fact have a finite subcover:
\[B_{x_1,2r_1}, ..., B_{x_n, 2r_n}\]
Choose $\delta = \min \{r_i\}$. Now for all $x \in K$, it belongs to one of the $B_{x_k, 2r_k} \subset U_a$.\\\
Then we claim $x \in B_{x, \delta} \subset B_{x_k, 2r_k} \subset U_a$. To do this, we need to verify $B_{x, \delta} \subset B_{x_k, 2r_k}$. Indeed, for all $y \in B_{x, \delta}$, we have that
\[d(y, x_k) \leq d(y, x) + d(x, x_k) \leq \delta +  \]
\end{proof}

To apply this lemma in our context, we take $K = [a, b]$ and for all $s \in [a, b]$, we define $U_s = \gamma^{-1}(D_{\gamma(s), r(s)})$, where $r(s)$ is the radius of convergence of $\gamma(s)$ under the power-series. Then we can apply the Lebesgue's Number Lemma.

\begin{question}
Is the integral well-defined up to two different splitting?
\end{question}

Yes, the idea is that given two splitting on the interval, one can join them using a refinement by taking smaller intervaks of both of them and used the associated antiderivative from either original splittings.

\begin{definition}
    Let $\gamma_0, \gamma_1: [a, b] \to \Omega$ be continuous. We say $\gamma_0$ is \textbf{homotopy equivalent} to $\gamma_1$ if there exists a continuous function $\Gamma: [a, b] \times [0, 1] \to \Omega$ such that $\Gamma(s, 0) = \gamma_0(s)$ and $\gamma(s, 1) = \gamma_1(s)$ for all $s \in [a, b]$.
\end{definition}

we will also assume that either:
        \begin{itemize}
            \item All pathes are closed, for all $t$
            \[\Gamma(a, t) = \Gamma(b, t)\]
            \item OR Endpoints are fixed
            \[\Gamma(a, t) = \gamma_0(a) = \gamma_1(b)\]
            \[\Gamma(b, t) = \gamma_0(b) = \gamma_1(b)\]
        \end{itemize}

\begin{theorem}
If $\gamma_0, \gamma_1$ are homotopy equivalent in $\Omega$ and $f \in Hol(\Omega)$, then
\[\int_{\gamma_0} f(z) dz = \int_{\gamma_1} f(z) dz\]
\end{theorem}

\begin{remark}
In a simply connected domain, any two pathes are homotopy equivalent. In otherwords, the path of integration is irrelevant.
\end{remark}

\newpage

\section{Lecture 8}

\subsection{Homotopy Invariance of Integrals - Continued}

\begin{theorem}
If $\gamma_0, \gamma_1$ are homotopy equivalent in $\Omega$ and $f \in Hol(\Omega)$, then
\[\int_{\gamma_0} f(z) dz = \int_{\gamma_1} f(z) dz\]
\end{theorem}

\begin{proof}
Let $\Gamma$ be the homotopy equivalence function. For all $z_0 \in \Omega$, let $D_{z_0}$ be a disc centered at $z_0$ small enough such that $f$ can be expressed as a power-series on it, define
\[U_{z_0} = \Gamma^{-1}(D_{z_0})\]
Then $\{U_{z_0}\}$ will be an open cover of $R \coloneqq [a, b] \times [0, 1]$, which is a compact metric space. Apply Lebesgue's Number Lemma, we find $\delta > 0$ such that, we can split $R$ into smaller rectangles $R_k$ where each $diam(R_k) < \delta$.\\\\
The Lebesgue Number Lemma tells us that, for each $R_k$, $\Gamma(cl(R_k)) \subset D_{z}$ for some $z$. Since $f$ is primitive on $D_z$, we have that
\[\int_{\Gamma|_{\partial R_k}} f(z) dz = 0\]
Putting the small rectangles together (Green's Theorem style), the inner edges cancel out, so we have that
\[\int_{\Gamma|_{\partial R}} f(z) dz = 0\]
Now consider the pathes $\ell_1 = \{a\} \times [0, 1]$ and $\ell_2 = \{b\} \times [0, 1]$, we claim that
\[\int_{\Gamma|_{\ell_1 + \ell_2}} f(z) dz = 0\]
Indeed, if endpoints are fixed, both paths are constant (stays at same point). If all path are closed, then this is the same path in opposite directions.\\\\
Thus, we only have to integrate over the horizontal pathes:
\[\int_{\partial R} f(z) dz = 0 = \int_{\gamma_0} f(z) dz - \int_{\gamma_1} f(z) dz\]
\end{proof}

\begin{definition}
    A set $\Omega$ is \textbf{simply connected} if any closed loop in $\Omega$ is homotopy equivalent to the constant path. This is equivalent to saying, for any pathes $\gamma_0, \gamma_1$, $\gamma_0(a) = \gamma_1(a) = z_0$, $\gamma_0(b) = \gamma_1(b) = z_1$, are homotopy equivalent.
\end{definition}

\begin{remark}
If $\Omega$ is simply connected domain, then
\[\int_{z_0}^z_1 f(z) dz\]
does not depend on the path specified.
\end{remark}

\begin{definition}
    Let $\Omega$ be simply connected and $f \in Hol(\Omega)$. Suppose $f(z) \neq 0$ for all $z \in \Omega$.\\\\
    Fix some $z_0 \in \Omega$, and consider
    \[a_0 \text{ such that } f(z_0) = e^{a_0}\]
    We can find $a_0$ as
    \[Re(a_0) = \log |f(z_0)|, Im(a_0) = arg\ f(z_0)\]
    Then we define
    \[\log f(z) \coloneqq a_0 + \int_{z_0}^z \frac{f'(\xi)}{f(\xi)} d\xi\]
\end{definition}

Show that $\log f(z)$ aligns with the global definition of the complex logarithm.

\begin{proof}
Exercise. The idea is to denote $\varphi(z) = a_0 + \int_{z_0}^z \frac{f'(\xi)}{f(\xi)} d\xi$ and show that
\[(f(z) e^{-y(z)})' = 0\]
and realize that their product must be $1$.
\end{proof}

\mattie{explain motivation later}
\begin{definition}
    What is $f(z)^{\alpha}$? We define
    \[f(z)^{\alpha} = e^{\alpha \log(f(z))}\]
    This is defined when $f \in Hol(\Omega)$, $f(z) \neq 0$ on all of $\Omega$, and $\Omega$ is simply connected.
\end{definition}

In a simply connected domain, the branch of the logarithm, it is enough to be determined by which $a_0$ you choose.

\subsection{Laurent Series}

Suppose $f$ is holomorphic on $\{z : a < |z - z_0| < A\}$, where we require $a \geq 0$ and $A \leq \infty$.

\begin{theorem}
If $f \in Hol\{z : a < |z - z_0| < A\}$, then $f$ can be represented as
\[f(z) = \sum_{n \in \Zbb} a_n (z - z_0)^n\]
, where we have that
\[a_n = \frac{1}{2\pi i} \int_{|\xi - z_0| = r} f(\xi) (\xi - z_0)^{-(n+1)} d\xi\]
, where $r$ is between $a < r < A$ (Note that for $\Zbb_+$, this is the same as the Taylor Power Series)
\end{theorem}

\begin{proof}
Without loss of generality, we can shift this to $z_0 = 0$.\\\\
Take $z$ such that $a < |z| < A$ and pick $r, R$ such that
\[a < r < |z| < R < A\]
Then consider the set
\[G \coloneqq \{z: r < |z| < R \}\]
Then Cauchy's Integral Formula gives
\begin{align*}
    f(z) &= \frac{1}{2\pi i} \int_{\partial G} \frac{f(\xi)}{\xi - z} d\xi\\
    &= \frac{1}{2\pi i} (\int_{|z| = R} \frac{f(\xi)}{\xi - z} d\xi - \int_{|z| = r} \frac{f(\xi)}{\xi - z} d\xi)\\
    &= \frac{1}{2\pi i} (I_1 - I_2)
\end{align*}
For $I_1$, we note that $|z| < |\xi| = R$, so
\begin{align*}
    I_1 &= \int_{|z| = R} \frac{f(\xi)}{\xi - z} d\xi\\
    &= \int_{|z| = R} \frac{f(\xi)}{\xi} \frac{1}{1 - \frac{z}{\xi}} d\xi\\
    &= \int_{|z| = R} f(\xi) \sum_{k = 0}^\infty \frac{z^k}{\xi^{k+1}}
\end{align*}
For $I_2$, we note that $|z| > |\xi| = r$, so
\begin{align*}
    I_2 &= \int_{|z| = r} \frac{f(\xi)}{\xi - z} d\xi\\
    &= \int_{|z| = r} \frac{-f(\xi)}{z} \frac{1}{1 - \frac{\xi}{z}} d\xi\\
    &= \int_{|z| = r} -f(\xi) \sum_{k = 0}^\infty \frac{\xi^k}{z^{k+1}}\\
    &= \int_{|z| = r} -f(\xi) \sum_{n = -\infty}^{-1} \frac{z^n}{\xi^{n+1}}\\ \tag*{Change of Variables}
\end{align*}
Since both series converge uniformly, we can integrate term by term and use Cauchy's Formula for Derivatives, rewriting both $I_1$ and $I_2$ out in series finishes the proof.
\end{proof}

Now we will consider a particular case of the Laurent Series!

\begin{definition}
    Let $f \in Hol(\Omega \setminus \{z_0\})$ where $z_0 \in \Omega$. In this case, we say $f$ has a singularity at $z_0$.\\\\
    Take $\delta$ small enough and $D_{z_0, \delta} \subset \Omega$, then the Laurent Series tells us
    \[f(z) = \sum_{n \in \Zbb} a_n (z - z_0)^n\]
    We say that
    \begin{itemize}
        \item $f$ has a \textbf{removable singularity} at $z_0$ if $a_n = 0$ for all $n < 0$. In this case,
        \[f(z) = \sum_{n \geq 0} a_n (z - z_0)^n, f(z_0) = a_0\]
        An example of such function would be $f(z) = \frac{sin(z)}{z}$ has removable singularity at $0$
        \item We say $f$ has a \textbf{pole at $z_0$} if $a_n \neq 0$ for finitely many $n < 0$. We say the \textbf{order of a pole} as
        \[\max \{n \geq 0: a_{-n} = 0\}\]
        \item We say that $f$ has an essential singularity if there exists infinitely many $n < 0$ such that $a_n \neq 0$.\\\\
        For example consider
        \[f(z) = e^{1/z} = \sum_{n = 0}^\infty \frac{z^{-n}}{n!}\]
        This has an essential singularity at $z = 0$.
    \end{itemize}
    These are the singularities we care about.
\end{definition}

\newpage
\section{Lecture 9}

Recall, let $f \in Hol(\Omega \setminus \{z_0\})$, where $z_0 \in \Omega$, we can write $f$ into a Laurent series
\[f(z) = \sum_{z \in \Zbb} a_n (z - z_0)^n, 0 < |z - z_0| < N\]
, and we say that $z_0$ is removable if $a_n = 0$ for all $n < 0$.

\begin{theorem}
$z_0$ is a removable singularity of $f$ if and only if there exists a neighborhood $z_0 \in U$ such that $f$ is bounded in $U \setminus \{z_0\}$.
\end{theorem}

\begin{proof}
If $f$ has a removable singularity, we can write it locally as
\[f(z) = \sum_{n \geq 0} a_n (z - z_0)^n\]
which has a positive radius of convergence and hence bounded in a neighborhood of $z_0$.\\\\
Conversely, suppose $f$ is bounded on $0 < |z - z_0| < \delta$. Then for all $n \geq 1$, we note that
\[a_{-n} = \frac{1}{2\pi i} \int_{|z - z_0| = r} f(z) (z - z_0)^{n-1} dz \]
As $n-1 \geq 0$ and $f$ is bounded, this integral is also bounded, so
\[|a_{-n}| \leq \frac{1}{2\pi} M (1) (2\pi r) = Mr\]
for all $0 < r < \delta$, we can shrink $r$ down and have that $a_{-n} = 0$.
\end{proof}

\begin{remark}
If $f(z) = O(\frac{1}{|z - z_0|})$, then $f$ has a removable singularity at $z_0$.
\end{remark}

We say $f$ has a \textbf{pole at $z_0$} if $a_n \neq 0$ for finitely many $n < 0$. We say the \textbf{order of a pole} as
        \[\max \{n \geq 0: a_{-n} = 0\}\]
        
\begin{theorem}
$z_0$ is a pole if and only if $\lim_{z \to z_0} |f(z)| = \infty$
\end{theorem}

\begin{proof}
Suppose $z_0$ is a pole of order $m$, then we can write
\[f(z) = \frac{g(z)}{(z - z_0)^m}, g(z_0) \neq 0\]
Hence we have that
\[\lim_{z \to z_0} |f(z)| = \lim_{z \to z_0} |\frac{g(z)}{(z - z_0)^m}| = \infty\]
Conversely, suppose $\lim_{z \to z_0} |f(z)| = \infty$, then we can find some $r > 0$ such that $|f(z)| > 1$ for all $z$ in $0 < |z - z_0| < r$.\\\\
Now consider $h(z) = \frac{1}{f(z)}$ on $D_{z_0, r} \setminus \{z_0\}$, then $h(z) \in Hol(D_{z_0, r} \setminus \{z_0\})$ and $\lim_{z \to z_0} h(z) = 0$ - so we can extend $h$ to the whole disk. Therefore it has to be the case that $|h(z)| < 1$, then by the previous theorem, this means $z_0$ is a removable singularity for $h$, so in fact $h$ is holomorphic on the whole disk.\\\\
Since $h(z_0) = 0$, we can find the smallest $m$ such that $h(z) = (z - z_0)^m h_0(z)$ but $h_0(z_0) \neq 0$. Now consider $g = \frac{1}{h}$, then we have that
\[f(z) = \frac{g(z)}{(z - z_0)^m}\]
Thus, $z_0$ is a pole of order $m$.
\end{proof}

We say that $f$ has an essential singularity if there exists infinitely many $n < 0$ such that $a_n \neq 0$.

\begin{theorem}[Casorati-Weierstrass Theorem]
If $f$ has an essential singularity at $z_0$, then for any neighborhood $U$ of $z_0$, $U \subset \Omega$, $f(U)$ is \textbf{dense} in $\Cbb$ (in other words, for all $w \in \Cbb$, there exists a sequence of $z_n$ such that $f(z_n) \to w$ as $z_n \to z_0$)
\end{theorem}

\begin{proof}
We will prove this using contradiction. Suppose there exists some neighborhood $U$ of $z_0$ such that $f(U)$ is not dense. Then there exists some $a \in \Cbb$ and $r > 0$ such that $D_{a, r} \cap f(U) = \emptyset$.\\\\
Now define $g(z) = \frac{1}{f(z) - a}$. Then clearly $g \in Hol(U)$ as the denominator is never $0$. We also have that $|g| < \frac{1}{|f(z) - a|} < \frac{1}{r}$. Moreover, we note that $g(z) \neq 0$ in $U \setminus \{z_0\}$ because $f$ is bounded?????. While $g(z_0)$ could be $0$, we will choose the smallest $m$ such that $g(z) = (z - z_0)^m g_0(z)$ and $g_0(z_0) \neq 0$.\\\\
Thus, $g_0(z) \neq 0$ on $U$. But we have that
\[f(z) = \frac{1}{g(z)} + a = \frac{1}{(z - z_0)^m g_0(z)} + a\]
, so $f$ has a removable singularity or some pole at $z_0$, hence a contradiction.
\end{proof}

\begin{definition}
    Suppose $f$ has a singularity at $z_0$ and write
    \[f(z) = \sum_{n \in \Zbb} a_n (z - z_0)^n\]
    Then we define the \textbf{residue of $f$ at $z_0$} as $a_{-1}$ and denote is as $Res_{z_0}(f)$ or $res(f, z_0)$
\end{definition}

\begin{remark}
If $z_0$ is a pole of order $1$, then
\[res(f, z_0) = \lim_{z \to z_0} (z - z_0)f(z)\]
\end{remark}

\begin{theorem}[Cauchy's Residue Theorem]
Let $G$ be a bounded domain with $\partial G \in PC^1$ and $\overline{G} \subset \Omega$. Let $z_1, ..., z_n \in G$ and $f \in Hol(\Omega \setminus \{z_1, ..., z_n\})$, then
\[\int_{\partial G} f(z) dz = 2\pi i \sum_{k = 1}^n Res(f, z_k)\]
\end{theorem}

\begin{proof}
Let $D_k$ be small disks around each $z_k$ and consider $\Tilde{G} = G \setminus \bigcup D_k$. Note that $f(z)$ is holomorphic on $\Tilde{G}$, so
\[\partial_{\partial \Tilde{G}} f(z) dz = 0\]
On the other hand, we also have that $\partial \Tilde{G} = \partial G - \bigcup \partial D_k$, so in other words
\[\int_{\partial G} f(z) dz = \sum_k \int_{\partial D_k} f(z) dz\]
Write $f$ as a Laurent Series, then every term except for the $-1$ term is primitive and thus evaluate to $0$, so we are left with:
\[\int_{\partial G} f(z) dz = 2\pi i \sum_{k = 1}^n Res(f, z_k)\]
\end{proof}

\end{document}
